\documentclass[12pt]{article}

\usepackage{geometry}
\usepackage{fancyhdr}
\usepackage{extramarks}
\usepackage{amsmath}
\usepackage{amsthm}
\usepackage{amsfonts}
\usepackage{amssymb}
\usepackage{tikz}
\usepackage[plain]{algorithm}
\usepackage{algpseudocode}
\usepackage{fancyhdr}
\usepackage{array}
\usepackage{wrapfig}
\usepackage{adjustbox}
\usepackage{enumitem}


\newlength{\strutheight}
\settoheight{\strutheight}{\strut}
\newtheorem{theorem}{Theorem}
\renewcommand\qedsymbol{$\blacksquare$}
\newcommand\setitemnumber[1]{\setcounter{enumi}{\numexpr#1--1\relax}}

\geometry{letterpaper,portrait,margin=1in}


\title{\large TITLE}
\author{\large Zachary Meyner}
\date{}

\begin{document}
\maketitle

\begin{enumerate}
    \item Prove (using the definition) $\lim\limits_{x \to 2} \frac{5x-3}{x-1} = 7$.
    \begin{proof}
        Let $\varepsilon > 0$ be given. Consider $\delta = \min(\frac{1}{2}, \frac{\varepsilon}{4})$ \\
        $\forall x$ s.t. $0 < |x-2| < \delta$
        \begin{align*}
            \bigg| \frac{5x-3}{x-1} - 7 \bigg| &= \bigg| \frac{5x-3-7x+7}{x-1} \bigg| \\
            &= \bigg| \frac{-2x+4}{x-1} \bigg| \\
            &= \bigg| \frac{-2(x-2)}{x-1} \bigg| \\
            &< 2\delta \bigg| \frac{1}{x-1} \bigg| \\
            &< \frac{2\delta}{\frac{1}{2}} && \text{(*)} \\
            &= 4\delta \\
            &= \varepsilon
        \end{align*}

        (*)
        \begin{gather*}
            \frac{-1}{2} < x-2 < \frac{1}{2}\\
            \frac{1}{2} < x-1 < \frac{3}{2} \\
            \therefore |x-1| = x-1 > \frac{1}{2}
        \end{gather*}
    \end{proof}

    \item Prove (using the definition) that $\lim\limits_{n \to \infty} \frac{3n-2n^2}{5-n} = \infty$.
    \begin{proof}
        Let $\alpha \in \mathbb{R}$, consider $K = \frac{\alpha+3}{2}$ \\
        Then $\forall n \geq K$
        \begin{align*}
            \frac{3n-2n^2}{5-n} &= \frac{2n^2-3n}{n-5} \\
            &> \frac{2n^2-3n}{n} \\
            &= 2n-3 \\
            &\geq 2K-3 \\
            &= \alpha
        \end{align*}
    \end{proof}

    \item Prove (using the definition) that $\lim\limits_{n \to \infty} \frac{n^3-5}{n-n^2} = -\infty$.
    \begin{proof}
        Let $\alpha \in \mathbb{R}$, consider $K = \max(5, -\alpha+1)$ \\
        Then $\forall n \geq K$
        \begin{align*}
            \frac{n^3-5}{n-n^2} &\leq \frac{n^3-5n}{n-n^2} && (n \geq 2) \\
            &= \frac{n^2-5}{1-n} \\
            &< \frac{n^2-5}{-n} && (n \geq 3) \\
            &= -n + \frac{5}{n} \\
            &\leq -n+1 && (n \geq 5) \\
            &\leq -K+1 \\
            &= \alpha
        \end{align*}
    \end{proof}

    \item Establish the proper divergence of the following sequence: $\Big(\frac{n^2}{\sqrt{n^3+1}} \Big)$.
    \[\lim_{n \to \infty} \frac{n^2}{\sqrt{n^3+1}} = \infty \]
    \begin{proof}
        Let $\alpha \in \mathbb{R}$, consider $K = 4\alpha^2$. \\
        Then $\forall n \geq K$
        \begin{align*}
            \frac{n^2}{\sqrt{n^3+1}} &\geq \frac{n^2}{\sqrt{n^3+n^3}} \\
            &= \frac{\sqrt{n}}{2} \\
            &\geq \frac{\sqrt{K}}{2} \\
            &= \alpha
        \end{align*}
    \end{proof}

    \item Prove the following limits.
    \begin{enumerate}
        \item $\lim\limits_{x \to 3} \frac{2}{1-x} = -1$
        \begin{proof}
            Let $\varepsilon > 0$ be given, consider $\delta = \min(1, \varepsilon) $, \\
            Then $\forall x$ s.t. $0 < |x-3| < \delta$
            \begin{align*}
                \bigg| \frac{2}{1-x} + 1 \bigg| &= \bigg| \frac{2+1-x}{1-x} \bigg| \\
                &= \bigg| \frac{x-3}{1-x} \bigg| \\
                &< \delta \bigg| \frac{1}{x-1} \bigg| \\
                &< \frac{\delta}{1} && \text{(*)} \\
                &= \varepsilon
            \end{align*}

            (*)
            \begin{gather*}
                -1 < x-3 < 1 \\
                1 < x-1 < 3 \\
                \therefore |x-1| = x-1 > 1
            \end{gather*}
        \end{proof}
        \item $\lim\limits_{x \to 1} \frac{x^2-2x+1}{x-2} = 0$
        \begin{proof}
            Let $\varepsilon > 0$ be given, consider $\delta = \min(\frac{1}{2}, \sqrt{\frac{\varepsilon}{2}}) $, \\
            then $\forall x$ s.t. $0 < |x-1| < \delta$
            \begin{align*}
                \bigg| \frac{x^2-2x+1}{x-2} \bigg| &= \bigg| \frac{{(x-1)}^2}{x-2} \bigg| \\
                &< \delta^2 \bigg| \frac{1}{x-2} \bigg| \\
                &< 2\delta^2 && \text{(*)} \\
                &= \varepsilon
            \end{align*}

            (*)
            \begin{gather*}
                \frac{-1}{2} < x-1 < \frac{1}{2} \\
                \frac{-3}{2} < x-2 < \frac{-1}{2} \\
                \frac{3}{2} > 2-x > \frac{1}{2} \\
                \therefore |x-2| = 2-x > \frac{1}{2}
            \end{gather*}
        \end{proof}
    \end{enumerate}
\end{enumerate}

\end{document}