\documentclass[12pt]{article}

\usepackage{geometry}
\usepackage{fancyhdr}
\usepackage{extramarks}
\usepackage{amsmath}
\usepackage{amsthm}
\usepackage{amsfonts}
\usepackage{amssymb}
\usepackage{tikz}
\usepackage[plain]{algorithm}
\usepackage{algpseudocode}
\usepackage{fancyhdr}
\usepackage{array}
\usepackage{wrapfig}
\usepackage{adjustbox}
\usepackage{enumitem}

\newlength{\strutheight}
\settoheight{\strutheight}{\strut}
\newtheorem{theorem}{Theorem}
\renewcommand\qedsymbol{$\blacksquare$}
\newcommand\setitemnumber[1]{\setcounter{enumi}{\numexpr#1-- -1\relax}}
\newcommand\Mydiv[2]{%
$\strut#1$\kern.25em\smash{\raise.3ex\hbox{$\big)$}}$\mkern-8mu
        \overline{\enspace\strut#2}$}

\geometry{letterpaper,portrait,margin=1in}


\title{\large Abstract Algebra Homework 9}
\author{\large Zachary Meyner}
\date{}

\begin{document}
\maketitle
\begin{enumerate}[label=\textbf{\arabic*}.]
	\setitemnumber{2}
	\item Compute each of the following.
	      \begin{enumerate}
		      \item $(5x^2+3x-4)+(4x^2-x+9)$ in $\mathbb{Z}_{12}[x]$ \\
		            $=(9x^2+2x+5) \mod{12}$
		      \item $(5x^2+4x-4)(4x^2-x+9)$ in $\mathbb{Z}_{12}[x]$ \\
		            $=20x^4+11x^3+25x^2+40x-36 = (8x^4+11x^3+x^2+4x) \mod{12}$
		      \item $(7x^3+3x^2-x) + (6x^2-8x+4)$ in $\mathbb{Z}_{9}[x]$ \\
		            $=(7x^3+4) \mod{9}$
		      \item $(3x^2+2x-4) + (4x^2+2)$ in $\mathbb{Z}_{5}[x]$ \\
		            $=(2x^2+2x+3) \mod{5}$
		      \item $(3x^2+2x-4)(4x^2+2)$ in $\mathbb{Z}_{5}[x]$ \\
		            $=12x^4+8x^3-10x^2+4x-8 = (2x^4+3x^3+4x+2) \mod{5}$
		      \item ${(5x^2+3x-2)}^2$ in $\mathbb{Z}_{12}[x]$ \\
		            $=25x^4+30x^3-11x^2-12x+4 = (x^4+6x^3+x^2+4) \mod{12}$
	      \end{enumerate}

	      \setitemnumber{3}
	\item Use the division algorithm to find $q(x)$ and $r(x)$ such that $a(x) = q(x)b(x) + r(x)$ with
	      $\deg r(x) < \deg b(x)$ for each of the following pairs of polynomials.
	      \begin{enumerate}
		      \item $a(x) = 5x^3+6x^2-3x+4$ and $b(x) = x-2$ in $\mathbb{Z}_{7}[x]$
		            \begin{align*}
			             & \qquad \quad 5x^2+16x+29                                   \\
			             & \text{\Mydiv{x-2}{5x^3+6x^2\ -\ 3x+ \ 4}}                  \\
			             & \quad \ \ \: \underline{-(5x^3-10x^2)}                     \\
			             & \qquad \quad \: \! 0x^3+16x^2 -3x                          \\
			             & \qquad \qquad \; \; \underline{-(16x^2-32x)}               \\
			             & \qquad \qquad \qquad \qquad \quad 29x+4                    \\
			             & \qquad \qquad \qquad \qquad \, \! \! \underline{-(29x-58)} \\
			             & \qquad \qquad \qquad \qquad \qquad \qquad 62
		            \end{align*}
		            $5x^3+6x^2-3x+4 = (x-2)(6x^2+16x+29) + 62$ \\
		            $=[(x-2)(5x^2+2x+1) + 6] \mod{7}$

		      \item $a(x) = 6x^4-2x^3+x^2-3x+1$ and $b(x) = x^2+x-2$ in $\mathbb{Z}_{7}[x]$
		            \begin{align*}
			             & \qquad \qquad \quad \; 6x^2-8x+21                               \\
			             & \text{\Mydiv{x^2+x-2}{6x^4-2x^3 + \ \quad \! x^2-3x+1}}         \\
			             & \qquad \qquad \, \underline{-(6x^4+6x^3-12x^2)}                 \\
			             & \qquad \qquad \qquad \; \; \; -8x^3+13x^3-3x                    \\
			             & \qquad \qquad \qquad \, \underline{-(-8x^3-8x^2+16x)}           \\
			             & \qquad \qquad \qquad \qquad \qquad \ \, 21x^2-19x+1             \\
			             & \qquad \qquad \qquad \qquad \quad \ \underline{-(21x^2+21x-42)} \\
			             & \qquad \qquad \qquad \qquad \qquad \qquad \quad -40x+43
		            \end{align*}
		            $6x^4-2x^3+x^2-3x+1 = (x^2+x-2)(6x^2-8x+21)+(-40x+43)$ \\
		            $=(x^2+x-2)(6x^2-x)+(2x+1)$

		      \item $a(x) = 4x^5-x^3+x^2+4$ and $b(x) = x^3-2$ in $\mathbb{Z}_{5}[x]$
		            \begin{align*}
			             & \qquad \quad \ \: \! 4x^2-1                       \\
			             & \text{\Mydiv{x^3-2}{4x^5 \ - \ x^3 \, + \ x^2+4}} \\
			             & \qquad \ \underline{-(4x^5+0x^3-8x^2)}            \\
			             & \qquad \qquad \quad \; \, -x^3+9x^2+4             \\
			             & \qquad \qquad \ \ \underline{-(-x^3+0x^2+2)}      \\
			             & \qquad \qquad \qquad \qquad \quad 9x^2-2
		            \end{align*}
		            $4x^5-x^3+x^2+4 = (x^3-2)(4x^2-1) + (9x^2-2)$ \\
		            $=(x^3-2)(4x^2-1)+(4x^2-2) \mod{5}$

		      \item $a(x) = x^5+x^3-x^2-x$ and $b(x) = x^3+x$ in $\mathbb{Z}_{2}[x]$
		            \begin{align*}
			             & \qquad \quad \ \: \! x^2            \\
			             & \text{\Mydiv{x^3+x}{x^5+x^3-x^2-x}} \\
			             & \qquad \ \underline{-(x^5+x^3)}     \\
			             & \qquad \qquad \qquad 0-x^2-x
		            \end{align*}
		            $x^5+x^3-x^2-x = (x^3+x)(x^2) + (-x^2-x) \mod{2}$
	      \end{enumerate}
          
          \setitemnumber{5}
          \item Find all of the zeros for each of the following polynomials.
          \begin{enumerate}
              \item $5x^3+4x^2-x+9$ in $\mathbb{Z}_{12}[x]$ \\
              None

              \item $3x^3-4x^2-x+4$ in $\mathbb{Z}_{5}[x]$ \\
              $x=2$

              \item $5x^4+2x^2-3$ in $\mathbb{Z}_{7}[x]$ \\
              $x = 3,4$

              \item $x^3+x+1$ in $\mathbb{Z}_{2}[x]$ \\
              None
          \end{enumerate}
          
          \setitemnumber{8}
          \item Which of the following polynomials are irreducible over $\mathbb{Q}[x]$.
          \begin{enumerate}
              \item $x^4-2x^3+2x^2+x+4 = (x^2-3x+5)(x^2+x+1)$. So it is not irreducible.
              \item $x^4-5x^3+3x-2$. It has no roots from the rational roots theorem, so if it's will 
              be so by quadratics. According to Gauss's Lemma it can written be as 
              \[x^4-5x^3+3x-2 = (x^2+ax+b)(x^2+cx+d)\]
              where $a,b,c,d \in \mathbb{Z}$.
              We know that
              \begin{align*}
                  -5 &= a+c \\
                  0 &= b+d+ac \\
                  3 &= ad+bc \\
                  -2 &= bd
              \end{align*}
              WLOG we have either $b=-2, d = 1$ or $b=2, d=-1$ \\
              When $b=-2$ and $d=1$ then we know
              \begin{align*}
                  -5 &= a+c \\
                  3 &= a-2c
              \end{align*}
              Which would mean 
              \[-8 = 3c\]
              Which has no integer solution, so it is irreducible for this case. \\
              When $b=2$ and $d=-1$ then we have
              \begin{align*}
                  -5 &= a+c \\
                  3 &= -a+2c
              \end{align*}
              Which would mean
              \[-2=3c\]
              Which has no integer solution. \\
              Therefore the polynomial is irreducible.

              \item $3x^5-4x^3-6x^2+6$ \\
              Let $p = 2$. Then $p|6, \ p|-6, \ p|-4, \ p\nmid 3$ and $p^2\nmid 6$, so by Einstein's Criterion 
              the function is irreducible over $\mathbb{Q}$.
              
              \item $5x ^5-6x^4-3x^2+9x-15$ \\
              Let $p = 3$. Then $p|15, \ p|9, \ p|-3, \ p|-6, p\nmid 5$ and $p^2\nmid 15$, so by Einstein's 
              Criterion the function is irreducible over $\mathbb{Q}$.
          \end{enumerate}
          \setitemnumber{17}
          \item Let $F$ be a field and $a \in F$. If $p(x) \in F[x]$, show that $p(a)$ is the remainder obtained 
          when $p(x)$ is dived by $x-a$.
          \begin{proof}
              According to the division algorithm if $p(x)$ is divided by $x-a$ then \\
              $\exists q(x),r(x) \in F[x]$ s.t. $p(x) = (x-a)q(x) + r(x)$ with \\
              $\deg(r(x)) < \deg(x-a) = 1$ or $r(x) = 0$. Then 
              \begin{align*}
                  p(a) &= (a-a)q(a) + r(a) \\
                  &= 0q(a) + r(a) \\
                  &= r(a)
              \end{align*}
              Therefore the remaineder $r(a) = p(a)$.
          \end{proof}

\end{enumerate}

\end{document}